Veritas.Verifier.Global.fsti
@@ -57,6 +57,20 @@ let g_add_set (gl: verifiable_log): mset ms_hashfn_dom =
 val lemma_g_hadd_correct (gl: verifiable_log):
   Lemma (hadd gl = ms_hashfn (g_add_seq gl))
 
+(* mapping from blum_add entries in verifier log to the index in add seq *)
+val add_set_map (gl: verifiable_log) (ii: sseq_index gl {is_blum_add (indexss gl ii)}):
+  (j: seq_index (g_add_seq gl){index (g_add_seq gl) j = blum_add_elem (indexss gl ii)})
+
+(* inverse mapping from add_seq to the blum add entries in the verifier logs *)
+val add_set_map_inv (gl: verifiable_log) (j: seq_index (g_add_seq gl)):
+  (ii: sseq_index gl {is_blum_add (indexss gl ii) /\ 
+                      add_set_map gl ii = j})
+
+val lemma_add_set_map_into (gl: verifiable_log) (ii1 ii2: sseq_index gl):
+  Lemma (requires (is_blum_add (indexss gl ii1) /\
+                   is_blum_add (indexss gl ii2)))
+        (ensures (ii1 <> ii2 ==> add_set_map gl ii1 <> add_set_map gl ii2))
+
 (* a single sequence containing all the blum evicts *)
 val g_evict_seq (gl: verifiable_log): seq ms_hashfn_dom 
 
